@prefix : <http://w3id.org/dakikg#> .
@prefix rdfs: <http://www.w3.org/2000/01/rdf-schema#> .
@prefix owl: <http://www.w3.org/2002/07/owl#> .
@prefix xsd: <http://www.w3.org/2001/XMLSchema#> .
@prefix dcterms: <http://purl.org/dc/terms/> .

# DAKI-KG

<http://w3id.org/dakikg#> a owl:Ontology ;
    dcterms:title "DAKI-KG vocabulary" ;
    dcterms:creator "Romy Vos" ;
    dcterms:creator "Iacopo Vagliano" ;
    dcterms:creator "Cornelis Boersma" ;
    dcterms:creator "Frank van Harmelen" ;
    dcterms:creator "Annette ten Teije" ;
    dcterms:creator "Joanna E Klopotowska" ;
    dcterms:description "An ontology defining custom classes and properties used in DAKI-KG" ;
    dcterms:license <https://creativecommons.org/licenses/by-nc-sa/4.0/>;
    rdfs:seeAlso <https://github.com/romy-vos/daki-kg#readme> ;
    owl:versionIRI <https://w3id.org/dakikg/1.0> ;
    owl:versionInfo "Version 1.0 (12-2025)" .

# CLASSES

:Drug a rdfs:Class ;
    rdfs:label "Drug" ;
    rdfs:comment "Represents a low-level ATC code (3rd level or lower)." .

:DrugClass a rdfs:Class ;
    rdfs:label "Drug Class" ;
    rdfs:comment "Represents a 2nd-level ATC code." .

:NephrotoxicConcept a rdfs:Class ;
    rdfs:label "Nephrotoxic Concept" ;
    rdfs:comment "Represents the combination of SNOMED CT terms that are in the AKIConcepts and CKDConcepts." .

:AKIConcept a rdfs:NephrotoxicConcept ;
    rdfs:label "AKI Concept" ;
    rdfs:comment "Groups SNOMED CT terms relevant to Acute Kidney Injury (AKI)." ;
    rdfs:subClassOf :NephrotoxicConcept .

:CKDConcept a rdfs:Class ;
    rdfs:label "CKDConcept" ;
    rdfs:comment "Groups SNOMED CT terms relevant to Chronic Kidney Disease (CKD)." ;
    rdfs:subClassOf :NephrotoxicConcept .

:DDI a rdfs:Class ;
    rdfs:label "Drug-Drug Interaction (DDI)" ;
    rdfs:comment "Represents a drug-drug interaction group." .

# OBJECT PROPERTIES

:hasAdverseEvent a owl:ObjectProperty ;
    rdfs:label "has adverse event" ;
    rdfs:comment "Describes an adverse event of a drug." .

:isIndicatedFor a owl:ObjectProperty ;
    rdfs:label "is indicated for" ;
    rdfs:comment "Describes a therapeutic use (indication) of a drug." .

:isContraIndicatedFor a owl:ObjectProperty ;
    rdfs:label "is contraindicated for" ;
    rdfs:comment "Describes a contraindication of a drug." .

:isRiskFactorFor a owl:ObjectProperty ;
    rdfs:label "is risk factor for" ;
    rdfs:comment "Describes a risk factor for a disease. Both drugs and clinical findings can be a risk factor." .

:hasInteractionWith a owl:ObjectProperty ;
                    a owl:SymmetricProperty ;
    rdfs:label "has interaction with" ;
    rdfs:comment "Describes an interaction between two drugs." .

# DATATYPE PROPERTIES

:hasNephrotoxicEffect a owl:DatatypeProperty ;
    rdfs:label "has nephrotoxic effect" ;
    rdfs:comment "Describes whether the effect of a drug-drug interaction is potentially nephrotoxic. 0=no effect, 1=higher risk, 2=potentially nephrotoxic." ;
    rdfs:range xsd:integer .

:requiresAction a owl:DatatypeProperty ;
    rdfs:label "requires action" ;
    rdfs:comment "Describes whether a drug-drug interaction requires any action." ;
    rdfs:range xsd:boolean .

# RDF STAR PROPERTIES

:hasFrequency a owl:AnnotationProperty ;
    rdfs:label "has frequency" ;
    rdfs:comment """Describes for a drug-adverse event triple the reported frequency.
Possible categories: 5 (very often), 4 (often), 3 (moderate), 2 (rare), 1 (very rare), -1 (unspecified).""" .

:isMemberOfInteraction a owl:AnnotationProperty ;
    rdfs:label "is member of interaction" ;
    rdfs:comment "Describes the link from an interaction triple to an interaction type." .